src/high/resources.v
@@ -8,7 +8,9 @@ From iris_named_props Require Import named_props.
 From self Require Import extra.
 From self.lang Require Import lang.
 From self.base Require Import primitive_laws.
-From self.high Require Import dprop lifted_modalities.
+From self.high Require Import dprop abstract_state lifted_modalities.
+From self.high Require Export abstract_state.
+From self.high.resources Require Export bumpers preorders abstract_history.
 
 Class nvmHighDeltaG := MkNvmHighDeltaG {
   (* "Global" ghost names *)
@@ -32,20 +34,9 @@ Definition predicateR {Σ} :=
   agreeR (positive -d> val -d> laterO (optionO (nvmDeltaG Σ -d> (dPropO Σ)))).
 Definition predicatesR {Σ} := authR (gmapUR loc (@predicateR Σ)).
 
-(* Resource algebras that for each location stores the encoded abstract states
-associated with each message/store. *)
-Definition encoded_abs_historyR := gmapUR time (agreeR positiveO).
-Definition enc_abs_histories := gmap loc (gmap time positive).
 
-Definition know_abs_historiesR :=
-  authR (gmapUR loc (gmapUR time (agreeR positiveO))).
-
-(* Resourcce algebra that stores the encoded preorder for each location. *)
-Definition relationO := leibnizO (positive → positive → Prop).
-Definition preordersR := authR (gmapUR loc (agreeR relationO)).
-
-Definition bumpersR :=
-  authR (gmapUR loc (agreeR (leibnizO (positive → option positive)))).
+(* Definition bumpersR := *)
+(*   authR (gmapUR loc (agreeR (leibnizO (positive → option positive)))). *)
 
 (* Resource algebra that contains all the locations that are _shared_. *)
 Definition shared_locsR := authR (gsetUR loc).
@@ -69,240 +60,36 @@ Class nvmFixedG Σ := NvmFixedG {
   nvmG_highG :> nvmHighFixedG Σ;
 }.
 
-Class AbstractState ST `{Countable ST} := {
-  abs_state_relation : relation2 ST;
-  abs_state_preorder :> PreOrder abs_state_relation;
-}.
-
-Instance abstract_state_sqsubseteq `{AbstractState ST} : SqSubsetEq ST :=
-  abs_state_relation.
-
 Global Instance discretizable_ghost_map_elem `{ghost_mapG Σ K V} ℓ γ v :
   own_discrete.Discretizable (ℓ ↪[γ] v).
 Proof. rewrite ghost_map_elem_eq /ghost_map_elem_def. apply _. Qed.
 
-(** We define a few things about the resource algebra that that we use to encode
-abstract histories. *)
-Section abs_history_lemmas.
-  Context `{nvmFixedG Σ, hGD : nvmDeltaG Σ}.
-  Context `{Countable ST}.
+(* Wrappers around ownership of resources that extracts the ghost names from [nvmDeltaG]. *)
 
-  Implicit Types
-    (abs_hist : gmap time ST) (ℓ : loc)
-    (enc_abs_hist : gmap time positive)
-    (abs_hists : gmap loc (gmap time positive)).
+Section ownership_wrappers.
+  Context `{nvmFixedG Σ, nD : nvmDeltaG Σ}.
 
-  Definition abs_hist_to_ra abs_hist : encoded_abs_historyR :=
-    (to_agree ∘ encode) <$> abs_hist.
+  Definition know_bumper `{AbstractState ST} ℓ bumper :=
+    own_know_bumper bumpers_name ℓ bumper.
 
-  Definition own_full_history_gname γ1 γ2 abs_hists : iProp Σ :=
-    ghost_map_auth γ1 1 abs_hists ∗
-    own γ2 (
-      ● ((λ m : gmap _ _, to_agree <$> m) <$> abs_hists) : know_abs_historiesR
-    ).
+  Definition know_preorder_loc `{Countable A} ℓ (preorder : relation2 A) : iProp Σ :=
+    own_know_preorder_loc preorders_name ℓ preorder.
 
-  Definition own_full_history abs_hists : iProp Σ :=
-    own_full_history_gname abs_history_name know_abs_history_name abs_hists.
+  Definition know_full_encoded_history_loc ℓ enc_abs_hist : iProp Σ :=
+    own_full_encoded_history_loc abs_history_name ℓ enc_abs_hist.
 
-  Definition know_full_history_loc ℓ abs_hist : iProp Σ :=
-    ℓ ↪[ abs_history_name ] (encode <$> abs_hist).
-
-  Definition know_full_encoded_history_loc
-             ℓ (abs_hist : gmap time positive) : iProp Σ :=
-    ℓ ↪[ abs_history_name ] abs_hist.
+  Definition know_full_history_loc `{Countable ST}
+             ℓ (abs_hist : gmap time ST) : iProp Σ :=
+    own_full_history_loc abs_history_name ℓ abs_hist.
 
   Definition know_frag_encoded_history_loc ℓ enc_abs_hist : iProp Σ :=
-    own know_abs_history_name (◯ {[ ℓ := to_agree <$> enc_abs_hist ]}).
+    own_frag_encoded_history_loc know_abs_history_name ℓ enc_abs_hist.
 
-  (* In this definition we store that decoding the stored encoded histry is
-  equal to our abstract history. This is weaker than strong the other way
-  around, namely that encoding our history is equal to the stored encoded
-  history. Storing this weaker fact makes the definition easier to show. This is
-  important for the load lemma where, when we load some state and we want to
-  return [know_store_lb] for the returned state. At that point we can
-  conclude that decoding the encoding gives a result but not that the encoding
-  is an encoding of some state. *)
-  Definition know_frag_history_loc ℓ (abs_hist : gmap time ST) : iProp Σ :=
-    ∃ enc,
-      ⌜decode <$> enc = Some <$> abs_hist⌝ ∗
-      (* ⌜enc = encode <$> abs_hist⌝ ∗ *)
-      know_frag_encoded_history_loc ℓ enc.
+  Definition know_frag_history_loc `{Countable ST}
+             ℓ (abs_hist : gmap time ST) : iProp Σ :=
+    own_frag_history_loc know_abs_history_name ℓ abs_hist.
 
-  Lemma own_full_history_gname_alloc h :
-    ⊢ |==> ∃ γ1 γ2,
-        own_full_history_gname γ1 γ2 h ∗
-        own γ2 (◯ ((λ m : gmap _ _, to_agree <$> m) <$> h) : know_abs_historiesR) ∗
-        [∗ map] k↦v ∈ h, k ↪[γ1] v.
-  Proof.
-    iMod (ghost_map_alloc h) as (new_abs_history_name) "[A B]".
-    iExists _. iFrame "A B".
-    setoid_rewrite <- own_op.
-    iMod (own_alloc _) as "$".
-    { apply auth_both_valid_2; last reflexivity.
-      intros k.
-      rewrite lookup_fmap.
-      destruct (h !! k); simpl; last done.
-      apply Some_valid.
-      intros k'.
-      rewrite lookup_fmap.
-      destruct (g !! k'); done. }
-    done.
-  Qed.
-
-  Lemma know_full_equiv ℓ abs_hist :
-    know_full_history_loc ℓ abs_hist ⊣⊢
-      know_full_encoded_history_loc ℓ (encode <$> abs_hist).
-  Proof. done. Qed.
-
-  Lemma know_frag_equiv ℓ abs_hist :
-    know_frag_encoded_history_loc ℓ (encode <$> abs_hist) ⊢
-    know_frag_history_loc ℓ abs_hist.
-  Proof.
-    rewrite /know_frag_history_loc /know_frag_encoded_history_loc.
-    iIntros "H".
-    iExists _. iFrame. iPureIntro.
-    apply map_eq. intros t.
-    rewrite !lookup_fmap.
-    destruct (abs_hist !! t); last done.
-    simpl. by rewrite decode_encode.
-  Qed.
-
-  Lemma abs_hist_to_ra_inj hist hist' :
-    abs_hist_to_ra hist' ≡ abs_hist_to_ra hist →
-    hist' = hist.
-  Proof.
-    intros eq.
-    apply: map_eq. intros t.
-    pose proof (eq t) as eq'.
-    rewrite !lookup_fmap in eq'.
-    destruct (hist' !! t) as [h|] eqn:leq, (hist !! t) as [h'|] eqn:leq';
-      try inversion eq'; auto.
-    simpl in eq'.
-    apply Some_equiv_inj in eq'.
-    apply to_agree_inj in eq'.
-    apply encode_inj in eq'.
-    rewrite eq'.
-    done.
-  Qed.
-
-  Lemma abs_hist_to_ra_agree hist hist' :
-    to_agree <$> hist' ≡ abs_hist_to_ra hist → hist' = encode <$> hist.
-  Proof.
-    intros eq.
-    apply: map_eq. intros t.
-    pose proof (eq t) as eq'.
-    rewrite !lookup_fmap in eq'.
-    rewrite lookup_fmap.
-    destruct (hist' !! t) as [h|] eqn:leq, (hist !! t) as [h'|] eqn:leq';
-      try inversion eq'; auto.
-    simpl in eq'. simpl.
-    apply Some_equiv_inj in eq'.
-    apply to_agree_inj in eq'.
-    f_equiv.
-    apply eq'.
-  Qed.
-
-  (** If you know the full history for a location and own the "all-knowing"
-  resource, then those two will agree. *)
-  Lemma own_full_history_agree ℓ hist hists :
-    own_full_history hists -∗
-    know_full_history_loc ℓ hist -∗
-    ⌜hists !! ℓ = Some (encode <$> hist)⌝.
-  Proof.
-    iIntros "[A _] B".
-    iApply (ghost_map_lookup with "[$] [$]").
-  Qed.
-
-  Lemma own_frag_history_agree ℓ (part_hist : gmap time ST) hists :
-    own_full_history hists -∗
-    know_frag_history_loc ℓ part_hist -∗
-    ⌜∃ hist, hists !! ℓ = Some (hist) ∧
-            (Some <$> part_hist) ⊆ (decode <$> hist)⌝.
-  Proof.
-    rewrite /own_full_history.
-    iIntros "[O A]".
-    iDestruct 1 as (enc) "[%eq K]".
-    iDestruct (own_valid_2 with "A K") as %[incl _]%auth_both_valid_discrete.
-    apply singleton_included_l in incl.
-    destruct incl as [hist' [look incl]].
-    rewrite lookup_fmap in look.
-    destruct (hists !! ℓ) as [hist|]. 2: { inversion look. }
-    simpl in look.
-    iExists hist.
-    iSplit; first done.
-    rewrite <- eq.
-    move: incl.
-    rewrite <- look.
-    rewrite Some_included_total.
-    rewrite -to_agree_fmap.
-    intros incl.
-    iPureIntro.
-    by apply map_fmap_mono.
-  Qed.
-
-  Lemma own_frag_history_agree_singleton ℓ t (s : ST) hists :
-    own_full_history hists -∗
-    know_frag_history_loc ℓ {[ t := s ]} -∗
-    ⌜∃ hist enc,
-      hists !! ℓ = Some hist ∧ hist !! t = Some enc ∧ decode enc = Some s⌝.
-  Proof.
-    iIntros "H1 H2".
-    iDestruct (own_frag_history_agree with "H1 H2") as %[hist [look H1]].
-    iExists hist. iPureIntro.
-    rewrite map_fmap_singleton in H1.
-    rewrite -> map_subseteq_spec in H1.
-    specialize H1 with t (Some s).
-    epose proof (H1 _) as H2.
-    Unshelve. 2: { rewrite lookup_singleton. done. }
-    apply lookup_fmap_Some in H2.
-    destruct H2 as (enc & eq & lookHist).
-    exists enc.
-    repeat split; done.
-  Qed.
-
-  Lemma own_full_history_alloc ℓ t encS (s : ST) hists hist :
-    hists !! ℓ = Some hist →
-    hist !! t = Some encS →
-    decode encS = Some s →
-    own_full_history hists ==∗
-    own_full_history hists ∗ know_frag_history_loc ℓ {[ t := s ]}.
-  Proof.
-    iIntros (look lookHist decEq) "[$ H2]".
-    rewrite /own_full_history /know_frag_history_loc.
-    iMod (own_update with "H2") as "[$ H]".
-    { apply (auth_update_dfrac_alloc _ _ {[ ℓ := {[ t := to_agree encS ]} ]}).
-      apply singleton_included_l.
-      eexists _.
-      rewrite lookup_fmap.
-      rewrite look.
-      simpl.
-      split; first reflexivity.
-      rewrite /abs_hist_to_ra.
-      apply Some_included_total.
-      apply singleton_included_l.
-      eexists _.
-      rewrite lookup_fmap.
-      rewrite lookHist.
-      simpl.
-      split; f_equiv. }
-    iExists {[ t := encS ]}.
-    rewrite /know_frag_encoded_history_loc.
-    rewrite !map_fmap_singleton.
-    rewrite decEq.
-    iFrame.
-    done.
-  Qed.
-
-  (* This lemma seems false :'( *)
-  (* Lemma own_frag_history_agree ℓ part_hist hists : *)
-  (*   own_full_history hists -∗ *)
-  (*   know_frag_history_loc ℓ part_hist -∗ *)
-  (*   ⌜∃ hist, hists !! ℓ = Some (encode <$> hist) ∧ part_hist ⊆ hist⌝. *)
-  (* Proof. w w *)
-  (*   iIntros "O K". *)
-  (* Admitted. *)
-
-End abs_history_lemmas.
+End ownership_wrappers.
 
 Section location_sets.
   Context `{nvmFixedG Σ}.
@@ -419,221 +206,6 @@ Section predicates.
   Qed.
 
 End predicates.
-
-(* (* For each location in the heap we maintain the following "meta data". *)
-(* For every location we want to store: A type/set of abstract events, its full *)
-(* abstract history, the invariant assertion. The abstract history maps *)
-(* timestamps to elements of the abstract events. *) *)
-(* Record loc_info := { *)
-(*   l_state : Type; *)
-(* (*   (* l_val : val; *) *) *)
-(* (*   l_ϕ : l_state → val → dProp Σ; *) *)
-(*   l_abstract_history : gmap nat l_state; *)
-(* (*   (* * Type class instances *) *) *)
-(*   l_sqsubseteq : SqSubsetEq l_state; *)
-(*   l_preorder : PreOrder (⊑@{l_state}); *)
-(*   (* We need countable to squash states into [positive] *) *)
-(*   l_eqdecision : EqDecision l_state; *)
-(*   l_countable : Countable l_state; *)
-(* }. *)
-
-(* Existing Instances l_eqdecision l_countable. *)
-
-(* Definition encode_loc_info {Σ} (l : (@loc_info Σ)):= *)
-(*   ((λ '(m, s), (m, encode s)) <$> (l_abstract_history l), *)
-(*    λ v s, (l_ϕ l $ v) <$> decode s). *)
-
-Definition lift2 {A B C} `{MBind M, MRet M, FMap M} (f : A → B → C) (am : M A) (bm : M B) :=
-  a ← am;
-  b ← bm;
-  mret (f a b).
-
-Definition mapply {A B} `{MBind M, FMap M} (mf : M (A → B)) (a : M A) :=
-  mf ≫= (λ f, f <$> a).
-
-(* This notation does not seem to work for some reason. *)
-(* Notation "<*>" := mapply (at level 61, left associativity). *)
-Notation "mf <*> a" := (mapply mf a) (at level 61, left associativity).
-
-Section preorders.
-  Context `{nvmFixedG Σ, hGD : nvmDeltaG Σ}.
-  Context `{Countable A}.
-
-  Implicit Type (preorders : gmap loc (relation2 positive)).
-
-  Definition encode_relation (R : relation2 A) : relation2 positive :=
-    λ (a b : positive), default False (R <$> decode a <*> decode b).
-
-  Lemma encode_relation_iff (R : relation2 A) (a b : A) :
-    R a b ↔ (encode_relation R) (encode a) (encode b).
-  Proof.
-    rewrite /encode_relation.
-    rewrite !decode_encode.
-    reflexivity.
-  Qed.
-
-  Definition map_to_agree preorders : gmapUR _ (agreeR relationO) :=
-    to_agree <$> preorders.
-
-  Definition own_all_preorders_gname γ preorders :=
-    own γ (● (map_to_agree preorders)).
-
-  Definition own_all_preorders preorders :=
-    own_all_preorders_gname preorders_name preorders.
-
-  Definition know_preorder_loc ℓ (preorder : relation2 A) : iProp Σ :=
-    own preorders_name (◯ ({[ ℓ := to_agree (encode_relation preorder) ]})).
-
-  Global Instance persistent_know_preorder_loc ℓ preorder :
-    Persistent (know_preorder_loc ℓ preorder).
-  Proof. apply _. Qed.
-
-  Lemma own_all_preorders_gname_alloc (preorders : gmap loc (relation2 positive)) :
-    ⊢ |==> ∃ γ, own_all_preorders_gname γ preorders ∗
-                own γ (◯ ((to_agree <$> preorders) : gmapUR _ (agreeR relationO))).
-  Proof.
-    setoid_rewrite <- own_op.
-    iApply own_alloc.
-    apply auth_both_valid_discrete. split; first done.
-    rewrite /map_to_agree.
-    apply (valid_to_agree_fmap (B := relationO) preorders).
-  Qed.
-
-  Lemma own_all_preorders_persist γ preorders :
-    own_all_preorders_gname γ preorders ==∗
-    own γ (●□ ((to_agree <$> preorders) : gmapUR _ (agreeR relationO))).
-  Proof. iApply own_update. apply auth_update_auth_persist. Qed.
-
-  Lemma auth_valid_to_agree_singleton_l {B}
-        dq (m : gmap loc (leibnizO B)) e (ℓ : loc) :
-    ✓ (●{dq} (to_agree <$> m : gmapUR _ (agreeR _)) ⋅
-       ◯ {[ℓ := to_agree e]}) →
-    m !! ℓ = Some e.
-  Proof.
-    intros [_ [incl _]]%auth_both_dfrac_valid_discrete.
-    move: incl.
-    rewrite singleton_included_l.
-    intros [y [eq incl]].
-    move: incl.
-    rewrite lookup_fmap in eq.
-    apply Some_equiv_eq in eq.
-    destruct eq as [y' [look' eq]].
-    rewrite -eq.
-    rewrite <- look'.
-    rewrite option_included_total.
-    intros [|(? & ? & [= ?] & [= ?] & incl)]; first done.
-    destruct (m !! ℓ) as [encOrder|]; last done.
-    simpl in *.
-    simplify_eq.
-    setoid_rewrite to_agree_included in incl.
-    f_equiv.
-    apply leibniz_equiv.
-    done.
-  Qed.
-
-  Lemma own_all_preorders_singleton_frag dq γ ℓ preorders preorder :
-    own γ (●{dq} (map_to_agree preorders)) -∗
-    own γ (◯ ({[ ℓ := to_agree (encode_relation preorder)]})) -∗
-    ⌜preorders !! ℓ = Some (encode_relation preorder)⌝.
-  Proof.
-    iIntros "auth frag".
-    iDestruct (own_valid_2 with "auth frag") as %V.
-    iPureIntro.
-    eapply auth_valid_to_agree_singleton_l.
-    apply V.
-  Qed.
-
-  Lemma orders_lookup ℓ order1 order2 (orders : gmap loc (relation2 positive)) :
-    orders !! ℓ = Some order1 →
-    own_all_preorders orders -∗
-    know_preorder_loc ℓ order2 -∗
-    ⌜order1 = encode_relation order2⌝.
-  Proof.
-    iIntros (look) "auth frag".
-    iDestruct (own_all_preorders_singleton_frag with "auth frag")
-      as %look'.
-    simplify_eq. done.
-  Qed.
-
-  Lemma orders_frag_lookup γ preorders (ℓ : loc) order :
-    preorders !! ℓ = Some order →
-    own γ (◯ (map_to_agree preorders)) -∗
-    own γ (◯ ({[ ℓ := to_agree order ]} : gmapUR _ (agreeR relationO))).
-  Proof.
-    intros look. f_equiv. simpl.
-    apply auth_frag_mono.
-    rewrite singleton_included_l.
-    eexists _.
-    rewrite lookup_fmap look.
-    naive_solver.
-  Qed.
-
-  (* If we know that two encoded values are related by en encoded relation, then
-  we can "recover" related unencoded values taht are related by the unencoded
-  relation. *)
-  Lemma encode_relation_related (R : relation2 A) ea eb :
-    (encode_relation R) ea eb →
-    ∃ a b, decode ea = Some a ∧ decode eb = Some b ∧ R a b.
-  Proof.
-    rewrite /encode_relation.
-    destruct (decode ea) as [|], (decode eb) as [|]; try done.
-    intros ?. eexists _, _. done.
-  Qed.
-
-  Lemma encode_relation_decode_iff (R : relation2 A) ea eb (a b : A) :
-    decode ea = Some a →
-    decode eb = Some b →
-    (encode_relation R) ea eb →
-    R a b.
-  Proof. rewrite /encode_relation. intros -> ->. done. Qed.
-
-End preorders.
-
-Section bumpers.
-  Context `{!nvmFixedG Σ, hGD : nvmDeltaG Σ}.
-  Context `{AbstractState ST}.
-
-  Definition know_bumper (ℓ : loc) (bumper : ST → ST) : iProp Σ :=
-    let encodedBumper e := encode <$> (bumper <$> decode e)
-    in ⌜∀ s1 s2, s1 ⊑ s2 → bumper s1 ⊑ bumper s2⌝ ∗
-       own bumpers_name ((◯ {[ ℓ := to_agree encodedBumper ]}) : bumpersR).
-
-  Definition own_all_bumpers_gname γ encoded_bumpers :=
-    own γ (● (to_agree <$> encoded_bumpers) : bumpersR).
-
-  Definition own_all_bumpers encoded_bumpers :=
-    own_all_bumpers_gname bumpers_name encoded_bumpers.
-
-  Lemma own_all_bumpers_gname_alloc bumpers :
-    ⊢ |==> ∃ γ, own_all_bumpers_gname γ bumpers ∗
-                own γ (◯ ((to_agree <$> bumpers) : gmapUR _ (agreeR _))).
-  Proof.
-    setoid_rewrite <- own_op.
-    iApply own_alloc.
-    apply auth_both_valid_discrete. split; first done.
-    apply valid_to_agree_fmap.
-  Qed.
-
-  Lemma own_all_bumpers_persist γ encoded_bumpers :
-    own_all_bumpers_gname γ encoded_bumpers ==∗
-    own γ (●□ ((to_agree <$> encoded_bumpers) : gmapUR _ (agreeR _))).
-  Proof. iApply own_update. apply auth_update_auth_persist. Qed.
-
-  Lemma bumpers_frag_lookup γ (bumpers : gmap loc (positive → option positive))
-        (ℓ : loc) (bumper : positive → option positive) :
-    bumpers !! ℓ = Some bumper →
-    own γ (◯ (to_agree <$> bumpers) : bumpersR) -∗
-    own γ (◯ {[ ℓ := to_agree bumper ]}).
-  Proof.
-    intros look. f_equiv. simpl.
-    apply auth_frag_mono.
-    rewrite singleton_included_l.
-    eexists _.
-    rewrite lookup_fmap look.
-    naive_solver.
-  Qed.
-
-End bumpers.
 
 Definition increasing_list `{SqSubsetEq ST} (ss : list ST) :=
   ∀ i j s s', i < j → (ss !! i = Some s) → (ss !! j = Some s') → s ≠ s' ∧ s ⊑ s'.
