src/base/primitive_laws.v
@@ -63,10 +63,6 @@ Instance nvm_baseG_to_heapG `{nvmBaseFixedG Σ, hGD : nvmBaseDeltaG Σ} :
   gen_meta_name := name_gen_meta (heap_names_name);
 |}.
 
-(** Get the largest time of any message in a given history. *)
-Definition max_msg (h : history) : time :=
-  max_list (elements (dom (gset time) h)).
-
 (**** Lemmas about [max_msg]. *)
 
 Lemma lookup_max_msg (hist : history) :
@@ -111,23 +107,6 @@ Proof.
   apply max_list_not_elem_of_gt.
   lia.
 Qed.
-
-(** Convert a [store] to a [view] by taking the largest time for of any message
-for each location. We call this the "lub view" b.c., in an actual execution this
-view will be the l.u.b. of all the threads views. *)
-Definition max_view (heap : store) : view := MaxNat <$> (max_msg <$> heap).
-
-Definition hist_inv lub (hist : history) : Prop :=
-  (* Every history has an initial message. *)
-  is_Some (hist !! 0) ∧
-  (* Every view in every message is included in the lub view. *)
-  (map_Forall (λ t msg, msg.(msg_store_view) ⊑ lub) hist).
-
-(* Every store view in every message is included in [lub]. *)
-Definition valid_heap_lub lub (s : store) : Prop :=
-  map_Forall (λ _ hist, hist_inv lub hist) s.
-
-Definition valid_heap store : Prop := valid_heap_lub (max_view store) store.
 
 (* The state interpretation for the base logic. *)
 Definition nvm_heap_ctx `{hG : !nvmBaseFixedG Σ, hGD : nvmBaseDeltaG Σ} σ : iProp Σ :=
