src/high/abstract_state.v
@@ -1,0 +1,11 @@
+From stdpp Require Export countable.
+
+From self Require Import extra.
+
+Class AbstractState ST `{Countable ST} := {
+  abs_state_relation : relation2 ST;
+  abs_state_preorder :> PreOrder abs_state_relation;
+}.
+
+Instance abstract_state_sqsubseteq `{AbstractState ST} : SqSubsetEq ST :=
+  abs_state_relation.
