src/high/resources/abstract_history.v
@@ -1,0 +1,241 @@
+(* Resource algebra to store the abstract histories. *)
+
+From iris.algebra Require Import auth gmap.
+From iris.base_logic.lib Require Import own ghost_map.
+From iris.heap_lang Require Export locations.
+From iris.proofmode Require Import proofmode.
+
+From self.lang Require Import lang.
+From self Require Import extra.
+
+(* Resource algebras that for each location stores the encoded abstract states
+associated with each message/store. *)
+Definition encoded_abs_historyR := gmapUR time (agreeR positiveO).
+(* Definition enc_abs_histories := gmap loc (gmap time positive). *)
+
+Definition know_abs_historiesR :=
+  authR (gmapUR loc (gmapUR time (agreeR positiveO))).
+
+(** We define a few things about the resource algebra that that we use to encode
+abstract histories. *)
+Section abs_history_lemmas.
+  Context `{!ghost_mapG Σ loc (gmap time positive), inG Σ know_abs_historiesR}.
+  Context `{Countable ST}.
+
+  Implicit Types
+    (abs_hist : gmap time ST) (ℓ : loc)
+    (enc_abs_hist : gmap time positive)
+    (abs_hists : gmap loc (gmap time positive)).
+
+  Definition abs_hist_to_ra abs_hist : encoded_abs_historyR :=
+    (to_agree ∘ encode) <$> abs_hist.
+
+  (* If we own the full history then we own the authorative view of both the
+  resource algebras. *)
+  Definition own_full_history γ1 γ2 abs_hists : iProp Σ :=
+    ghost_map_auth γ1 1 abs_hists ∗
+    own γ2 (
+      ● ((λ m : gmap _ _, to_agree <$> m) <$> abs_hists) : know_abs_historiesR
+    ).
+
+  (* Definition own_full_history abs_hists : iProp Σ := *)
+  (*   own_full_history abs_history_name know_abs_history_name abs_hists. *)
+
+  Definition own_full_encoded_history_loc γ ℓ enc_abs_hist : iProp Σ :=
+    ℓ ↪[ γ ] enc_abs_hist.
+
+  Definition own_full_history_loc γ ℓ abs_hist : iProp Σ :=
+    ℓ ↪[ γ ] (encode <$> abs_hist).
+
+  Definition own_frag_encoded_history_loc γ ℓ enc_abs_hist : iProp Σ :=
+    own γ (◯ {[ ℓ := to_agree <$> enc_abs_hist ]}).
+
+  (* In this definition we store that decoding the stored encoded histry is
+  equal to our abstract history. This is weaker than strong the other way
+  around, namely that encoding our history is equal to the stored encoded
+  history. Storing this weaker fact makes the definition easier to show. This is
+  important for the load lemma where, when we load some state and we want to
+  return [know_store_lb] for the returned state. At that point we can
+  conclude that decoding the encoding gives a result but not that the encoding
+  is an encoding of some state. *)
+  Definition own_frag_history_loc γ ℓ (abs_hist : gmap time ST) : iProp Σ :=
+    ∃ enc,
+      ⌜decode <$> enc = Some <$> abs_hist⌝ ∗
+      (* ⌜enc = encode <$> abs_hist⌝ ∗ *)
+      own_frag_encoded_history_loc γ ℓ enc.
+
+  Lemma own_full_history_alloc h :
+    ⊢ |==> ∃ γ1 γ2,
+        own_full_history γ1 γ2 h ∗
+        own γ2 (◯ ((λ m : gmap _ _, to_agree <$> m) <$> h) : know_abs_historiesR) ∗
+        [∗ map] k↦v ∈ h, k ↪[γ1] v.
+  Proof.
+    iMod (ghost_map_alloc h) as (new_abs_history_name) "[A B]".
+    iExists _. iFrame "A B".
+    setoid_rewrite <- own_op.
+    iMod (own_alloc _) as "$".
+    { apply auth_both_valid_2; last reflexivity.
+      intros k.
+      rewrite lookup_fmap.
+      destruct (h !! k); simpl; last done.
+      apply Some_valid.
+      intros k'.
+      rewrite lookup_fmap.
+      destruct (g !! k'); done. }
+    done.
+  Qed.
+
+  Lemma own_full_equiv γ ℓ abs_hist :
+    own_full_history_loc γ ℓ abs_hist ⊣⊢
+      own_full_encoded_history_loc γ ℓ (encode <$> abs_hist).
+  Proof. done. Qed.
+
+  Lemma own_frag_equiv γ ℓ abs_hist :
+    own_frag_encoded_history_loc γ ℓ (encode <$> abs_hist) ⊢
+    own_frag_history_loc γ ℓ abs_hist.
+  Proof.
+    rewrite /own_frag_history_loc /own_frag_encoded_history_loc.
+    iIntros "H".
+    iExists _. iFrame. iPureIntro.
+    apply map_eq. intros t.
+    rewrite !lookup_fmap.
+    destruct (abs_hist !! t); last done.
+    simpl. by rewrite decode_encode.
+  Qed.
+
+  Lemma abs_hist_to_ra_inj hist hist' :
+    abs_hist_to_ra hist' ≡ abs_hist_to_ra hist →
+    hist' = hist.
+  Proof.
+    intros eq.
+    apply: map_eq. intros t.
+    pose proof (eq t) as eq'.
+    rewrite !lookup_fmap in eq'.
+    destruct (hist' !! t) as [h|] eqn:leq, (hist !! t) as [h'|] eqn:leq';
+      try inversion eq'; auto.
+    simpl in eq'.
+    apply Some_equiv_inj in eq'.
+    apply to_agree_inj in eq'.
+    apply encode_inj in eq'.
+    rewrite eq'.
+    done.
+  Qed.
+
+  Lemma abs_hist_to_ra_agree hist hist' :
+    to_agree <$> hist' ≡ abs_hist_to_ra hist → hist' = encode <$> hist.
+  Proof.
+    intros eq.
+    apply: map_eq. intros t.
+    pose proof (eq t) as eq'.
+    rewrite !lookup_fmap in eq'.
+    rewrite lookup_fmap.
+    destruct (hist' !! t) as [h|] eqn:leq, (hist !! t) as [h'|] eqn:leq';
+      try inversion eq'; auto.
+    simpl in eq'. simpl.
+    apply Some_equiv_inj in eq'.
+    apply to_agree_inj in eq'.
+    f_equiv.
+    apply eq'.
+  Qed.
+
+  (** If you know the full history for a location and own the "all-knowing"
+  resource, then those two will agree. *)
+  Lemma own_full_history_agree γ1 γ2 ℓ hist hists :
+    own_full_history γ1 γ2 hists -∗
+    own_full_history_loc γ1 ℓ hist -∗
+    ⌜hists !! ℓ = Some (encode <$> hist)⌝.
+  Proof.
+    iIntros "[A _] B".
+    iApply (ghost_map_lookup with "[$] [$]").
+  Qed.
+
+  Lemma own_frag_history_agree γ1 γ2 ℓ (part_hist : gmap time ST) hists :
+    own_full_history γ1 γ2 hists -∗
+    own_frag_history_loc γ2 ℓ part_hist -∗
+    ⌜∃ hist, hists !! ℓ = Some (hist) ∧
+            (Some <$> part_hist) ⊆ (decode <$> hist)⌝.
+  Proof.
+    rewrite /own_full_history.
+    iIntros "[O A]".
+    iDestruct 1 as (enc) "[%eq K]".
+    iDestruct (own_valid_2 with "A K") as %[incl _]%auth_both_valid_discrete.
+    apply singleton_included_l in incl.
+    destruct incl as [hist' [look incl]].
+    rewrite lookup_fmap in look.
+    destruct (hists !! ℓ) as [hist|]. 2: { inversion look. }
+    simpl in look.
+    iExists hist.
+    iSplit; first done.
+    rewrite <- eq.
+    move: incl.
+    rewrite <- look.
+    rewrite Some_included_total.
+    rewrite -to_agree_fmap.
+    intros incl.
+    iPureIntro.
+    by apply map_fmap_mono.
+  Qed.
+
+  Lemma own_frag_history_agree_singleton γ1 γ2 ℓ t (s : ST) hists :
+    own_full_history γ1 γ2 hists -∗
+    own_frag_history_loc γ2 ℓ {[ t := s ]} -∗
+    ⌜∃ hist enc,
+      hists !! ℓ = Some hist ∧ hist !! t = Some enc ∧ decode enc = Some s⌝.
+  Proof.
+    iIntros "H1 H2".
+    iDestruct (own_frag_history_agree with "H1 H2") as %[hist [look H1]].
+    iExists hist. iPureIntro.
+    rewrite map_fmap_singleton in H1.
+    rewrite -> map_subseteq_spec in H1.
+    specialize H1 with t (Some s).
+    epose proof (H1 _) as H2.
+    Unshelve. 2: { rewrite lookup_singleton. done. }
+    apply lookup_fmap_Some in H2.
+    destruct H2 as (enc & eq & lookHist).
+    exists enc.
+    repeat split; done.
+  Qed.
+
+  Lemma own_full_history_alloc_frag γ1 γ2 ℓ t encS (s : ST) hists hist :
+    hists !! ℓ = Some hist →
+    hist !! t = Some encS →
+    decode encS = Some s →
+    own_full_history γ1 γ2 hists ==∗
+    own_full_history γ1 γ2 hists ∗ own_frag_history_loc γ2 ℓ {[ t := s ]}.
+  Proof.
+    iIntros (look lookHist decEq) "[$ H2]".
+    rewrite /own_full_history /own_frag_history_loc.
+    iMod (own_update with "H2") as "[$ H]".
+    { apply (auth_update_dfrac_alloc _ _ {[ ℓ := {[ t := to_agree encS ]} ]}).
+      apply singleton_included_l.
+      eexists _.
+      rewrite lookup_fmap.
+      rewrite look.
+      simpl.
+      split; first reflexivity.
+      rewrite /abs_hist_to_ra.
+      apply Some_included_total.
+      apply singleton_included_l.
+      eexists _.
+      rewrite lookup_fmap.
+      rewrite lookHist.
+      simpl.
+      split; f_equiv. }
+    iExists {[ t := encS ]}.
+    rewrite /own_frag_encoded_history_loc.
+    rewrite !map_fmap_singleton.
+    rewrite decEq.
+    iFrame.
+    done.
+  Qed.
+
+  (* This lemma seems false :'( *)
+  (* Lemma own_frag_history_agree ℓ part_hist hists : *)
+  (*   own_full_history hists -∗ *)
+  (*   know_frag_history_loc ℓ part_hist -∗ *)
+  (*   ⌜∃ hist, hists !! ℓ = Some (encode <$> hist) ∧ part_hist ⊆ hist⌝. *)
+  (* Proof. w w *)
+  (*   iIntros "O K". *)
+  (* Admitted. *)
+
+End abs_history_lemmas.
