src/high/resources/bumpers.v
@@ -1,0 +1,57 @@
+From iris.algebra Require Import gmap auth.
+From iris.base_logic.lib Require Import own.
+From iris.heap_lang Require Export locations.
+From iris.proofmode Require Import proofmode.
+
+From self Require Import extra.
+From self.high Require Import abstract_state.
+
+Definition bumpersR :=
+  authR (gmapUR loc (agreeR (leibnizO (positive → option positive)))).
+
+Section bumpers.
+  Context `{inG Σ bumpersR}.
+  Context `{AbstractState ST}.
+
+  Definition own_know_bumper γ (ℓ : loc) (bumper : ST → ST) : iProp Σ :=
+    let encodedBumper e := encode <$> (bumper <$> decode e)
+    in ⌜∀ s1 s2, s1 ⊑ s2 → bumper s1 ⊑ bumper s2⌝ ∗
+       own γ ((◯ {[ ℓ := to_agree encodedBumper ]}) : bumpersR).
+
+  Definition own_all_bumpers γ encoded_bumpers :=
+    own γ (● (to_agree <$> encoded_bumpers) : bumpersR).
+
+  (* Definition own_all_bumpers encoded_bumpers := *)
+  (*   own_all_bumpers bumpers_name encoded_bumpers. *)
+
+  Lemma own_all_bumpers_alloc bumpers :
+    ⊢ |==> ∃ γ, own_all_bumpers γ bumpers ∗
+                own γ (◯ ((to_agree <$> bumpers) : gmapUR _ (agreeR _))).
+  Proof.
+    setoid_rewrite <- own_op.
+    iApply own_alloc.
+    apply auth_both_valid_discrete. split; first done.
+    apply valid_to_agree_fmap.
+  Qed.
+
+  Lemma own_all_bumpers_persist γ encoded_bumpers :
+    own_all_bumpers γ encoded_bumpers ==∗
+    own γ (●□ ((to_agree <$> encoded_bumpers) : gmapUR _ (agreeR _))).
+  Proof. iApply own_update. apply auth_update_auth_persist. Qed.
+
+  Lemma bumpers_frag_lookup γ (bumpers : gmap loc (positive → option positive))
+        (ℓ : loc) (bumper : positive → option positive) :
+    bumpers !! ℓ = Some bumper →
+    own γ (◯ (to_agree <$> bumpers) : bumpersR) -∗
+    own γ (◯ {[ ℓ := to_agree bumper ]}).
+  Proof.
+    intros look. f_equiv. simpl.
+    apply auth_frag_mono.
+    rewrite singleton_included_l.
+    eexists _.
+    rewrite lookup_fmap look.
+    naive_solver.
+  Qed.
+
+End bumpers.
+
