src/high/resources/preorders.v
@@ -1,0 +1,147 @@
+(* Resource algebra to store the preorders that are associated with each
+location. *)
+
+From iris.algebra Require Import auth gmap.
+From iris.base_logic.lib Require Import own.
+From iris.heap_lang Require Export locations.
+From iris.proofmode Require Import proofmode.
+
+From self Require Import extra.
+
+(* Resourcce algebra that stores the encoded preorder for each location. *)
+Definition relationO := leibnizO (positive → positive → Prop).
+Definition preordersR := authR (gmapUR loc (agreeR relationO)).
+
+Section preorders.
+  Context `{inG Σ preordersR}.
+  Context `{Countable A}.
+
+  Implicit Type (preorders : gmap loc (relation2 positive)).
+
+  Definition encode_relation (R : relation2 A) : relation2 positive :=
+    λ (a b : positive), default False (R <$> decode a <*> decode b).
+
+  Lemma encode_relation_iff (R : relation2 A) (a b : A) :
+    R a b ↔ (encode_relation R) (encode a) (encode b).
+  Proof.
+    rewrite /encode_relation.
+    rewrite !decode_encode.
+    reflexivity.
+  Qed.
+
+  Definition map_to_agree preorders : gmapUR _ (agreeR relationO) :=
+    to_agree <$> preorders.
+
+  Definition own_all_preorders γ preorders :=
+    own γ (● (map_to_agree preorders)).
+
+  (* Definition own_all_preorders preorders := *)
+  (*   own_all_preorders_gname preorders_name preorders. *)
+
+  Definition own_know_preorder_loc γ ℓ (preorder : relation2 A) : iProp Σ :=
+    own γ (◯ ({[ ℓ := to_agree (encode_relation preorder) ]})).
+
+  (* Global Instance persistent_know_preorder_loc ℓ preorder : *)
+  (*   Persistent (know_preorder_loc ℓ preorder). *)
+  (* Proof. apply _. Qed. *)
+
+  Lemma own_all_preorders_gname_alloc (preorders : gmap loc (relation2 positive)) :
+    ⊢ |==> ∃ γ, own_all_preorders γ preorders ∗
+                own γ (◯ ((to_agree <$> preorders) : gmapUR _ (agreeR relationO))).
+  Proof.
+    setoid_rewrite <- own_op.
+    iApply own_alloc.
+    apply auth_both_valid_discrete. split; first done.
+    rewrite /map_to_agree.
+    apply (valid_to_agree_fmap (B := relationO) preorders).
+  Qed.
+
+  Lemma own_all_preorders_persist γ preorders :
+    own_all_preorders γ preorders ==∗
+    own γ (●□ ((to_agree <$> preorders) : gmapUR _ (agreeR relationO))).
+  Proof. iApply own_update. apply auth_update_auth_persist. Qed.
+
+  Lemma auth_valid_to_agree_singleton_l {B}
+        dq (m : gmap loc (leibnizO B)) e (ℓ : loc) :
+    ✓ (●{dq} (to_agree <$> m : gmapUR _ (agreeR _)) ⋅
+       ◯ {[ℓ := to_agree e]}) →
+    m !! ℓ = Some e.
+  Proof.
+    intros [_ [incl _]]%auth_both_dfrac_valid_discrete.
+    move: incl.
+    rewrite singleton_included_l.
+    intros [y [eq incl]].
+    move: incl.
+    rewrite lookup_fmap in eq.
+    apply Some_equiv_eq in eq.
+    destruct eq as [y' [look' eq]].
+    rewrite -eq.
+    rewrite <- look'.
+    rewrite option_included_total.
+    intros [|(? & ? & [= ?] & [= ?] & incl)]; first done.
+    destruct (m !! ℓ) as [encOrder|]; last done.
+    simpl in *.
+    simplify_eq.
+    setoid_rewrite to_agree_included in incl.
+    f_equiv.
+    apply leibniz_equiv.
+    done.
+  Qed.
+
+  Lemma own_all_preorders_singleton_frag dq γ ℓ preorders preorder :
+    own γ (●{dq} (map_to_agree preorders)) -∗
+    own γ (◯ ({[ ℓ := to_agree (encode_relation preorder)]})) -∗
+    ⌜preorders !! ℓ = Some (encode_relation preorder)⌝.
+  Proof.
+    iIntros "auth frag".
+    iDestruct (own_valid_2 with "auth frag") as %V.
+    iPureIntro.
+    eapply auth_valid_to_agree_singleton_l.
+    apply V.
+  Qed.
+
+  Lemma orders_lookup γ ℓ order1 order2 (orders : gmap loc (relation2 positive)) :
+    orders !! ℓ = Some order1 →
+    own_all_preorders γ orders -∗
+    own_know_preorder_loc γ ℓ order2 -∗
+    ⌜order1 = encode_relation order2⌝.
+  Proof.
+    iIntros (look) "auth frag".
+    iDestruct (own_all_preorders_singleton_frag with "auth frag")
+      as %look'.
+    simplify_eq. done.
+  Qed.
+
+  Lemma orders_frag_lookup γ preorders (ℓ : loc) order :
+    preorders !! ℓ = Some order →
+    own γ (◯ (map_to_agree preorders)) -∗
+    own γ (◯ ({[ ℓ := to_agree order ]} : gmapUR _ (agreeR relationO))).
+  Proof.
+    intros look. f_equiv. simpl.
+    apply auth_frag_mono.
+    rewrite singleton_included_l.
+    eexists _.
+    rewrite lookup_fmap look.
+    naive_solver.
+  Qed.
+
+  (* If we know that two encoded values are related by en encoded relation, then
+  we can "recover" related unencoded values taht are related by the unencoded
+  relation. *)
+  Lemma encode_relation_related (R : relation2 A) ea eb :
+    (encode_relation R) ea eb →
+    ∃ a b, decode ea = Some a ∧ decode eb = Some b ∧ R a b.
+  Proof.
+    rewrite /encode_relation.
+    destruct (decode ea) as [|], (decode eb) as [|]; try done.
+    intros ?. eexists _, _. done.
+  Qed.
+
+  Lemma encode_relation_decode_iff (R : relation2 A) ea eb (a b : A) :
+    decode ea = Some a →
+    decode eb = Some b →
+    (encode_relation R) ea eb →
+    R a b.
+  Proof. rewrite /encode_relation. intros -> ->. done. Qed.
+
+End preorders.
